io/DM.IO.fst
@@ -5,9 +5,10 @@ open ExtraTactics
 
 open Common
 open Free
-open Free.IO
-open Free.IO.Call
+open DMFree
 open Hist
+open Free.IO.Sig
+open Free.IO.Call
 
 (** The postcondition for an io computation is defined over the
 result (type: a) and local trace (type: trace).
@@ -20,108 +21,59 @@ The history is  in reverse chronology order.
 
 At the end of an io computation, the local trace is appended
 in reverse order to the history. **)
+unfold let io_wps (cmd:io_cmds) (arg:io_sig.args cmd) : hist #event (io_sig.res cmd arg) = fun p h ->
+  match cmd with
+  | _ -> io_pre cmd arg h /\ (forall r. p [convert_call_to_event cmd arg r] r)
 
-let rec io_interpretation #a
-  (m : io a)
-  (p : hist_post a) : Type0 =
-  match m with
-  | Return x -> p x []
-  | Call cmd args fnc -> (
-    forall res. (
-      io_interpretation (fnc res) (gen_post p cmd args res)))
-
-
-// REFINED COMPUTATION MONAD (repr)
-let io_irepr (a:Type) (wp:hist a) =
-  // TODO: more intuition about this? why does this look like a
-  // reader monad?
-  h:trace -> post:hist_post a ->
-    Pure (io a)
-      (requires (wp h post))
-      (ensures (fun (m:io a) -> io_interpretation m post))
-
-let io_ireturn (a : Type) (x : a) : io_irepr a (hist_return a x) =
-  fun _ _ -> io_return a x
-
-let io_ibind
-  (a b : Type)
-  (wp_v : hist a)
-  (wp_f: a -> hist b)
-  (v : io_irepr a wp_v)
-  (f : (x:a -> io_irepr b (wp_f x))) :
-  Tot (io_irepr b (hist_bind _ _ wp_v wp_f)) =
-  fun h p ->
-    let t = (io_bind a b
-        (v h (compute_post a b h wp_f p))
-        (fun x ->
-          assume (wp_f x h p);
-           f x h p)) in
-    assume (io_interpretation t p);
-    t
-
-unfold
-let isubcomp (a:Type) (wp1 wp2: hist a) (f : io_irepr a wp1) :
-  Pure (io_irepr a wp2)
-    (requires hist_ord wp2 wp1)
-    (ensures fun _ -> True) =
-  f
-
-unfold
-let i_if_then_else
-  (a : Type)
-  (wp1 wp2: hist a)
-  (f : io_irepr a wp1)
-  (g : io_irepr a wp2) (b : bool) :
-  Tot Type =
-  io_irepr a (hist_if_then_else wp1 wp2 b)
+let theta #a = theta #a #io_cmds #io_sig #event io_wps
+  
+let dm_io = dm io_cmds io_sig event io_wps
+let dm_io_return = dm_return io_cmds io_sig event io_wps
+let dm_io_bind = dm_bind io_cmds io_sig event io_wps
+let dm_io_subcomp = dm_subcomp io_cmds io_sig event io_wps
+let dm_io_if_then_else = dm_if_then_else io_cmds io_sig event io_wps
+let lift_pure_dm_io = lift_pure_dm io_cmds io_sig event io_wps
 
 total
 reifiable
 reflectable
-layered_effect {
-  IOwp : a:Type -> wp : hist a -> Effect
-  with
-       repr       = io_irepr
-     ; return     = io_ireturn
-     ; bind       = io_ibind
-
-     ; subcomp      = isubcomp
-     ; if_then_else = i_if_then_else
+effect {
+  IOwp (a:Type) (wp : hist #event a) 
+  with {
+       repr       = dm_io
+     ; return     = dm_io_return
+     ; bind       = dm_io_bind 
+     ; subcomp    = dm_io_subcomp
+     ; if_then_else = dm_io_if_then_else
+     }
 }
 
-let lift_pure_iowp
-  (a:Type)
-  (wp:pure_wp a)
-  (f:(eqtype_as_type unit -> PURE a wp)) :
-  Tot (io_irepr a (fun h p -> wp (fun r -> p r [])))
-  = fun h p -> let r = elim_pure f (fun r -> p r []) in io_return _ r
-
-sub_effect PURE ~> IOwp = lift_pure_iowp
+sub_effect PURE ~> IOwp = lift_pure_dm_io
 
 effect IO
+  (a:Type)
+  (pre : trace -> Type0)
+  (post : trace -> a -> trace -> Type0) =
+  IOwp a 
+    (fun (p:hist_post a) (h:trace) -> pre h /\ (forall lt (r:a). post h r lt ==> p lt r)) 
+
+effect IOPi
   (a:Type)
   (pi : monitorable_prop)
   (pre : trace -> Type0)
   (post : trace -> a -> trace -> Type0) =
-  IOwp a (fun (h:trace) (p:hist_post a) ->
-    pre h /\
-    (forall res lt. (
+  IO a
+    (requires pre)
+    (ensures (fun h r lt -> 
       enforced_locally pi h lt /\
-      post h res lt ==> p res lt)))
+      post h r lt))
 
 let static_cmd
   (cmd : io_cmds)
   (pi : monitorable_prop)
-  (argz : io_args cmd) :
-  IOwp
-    (io_resm cmd)
-    (fun h p ->
-      (** precondition **)
-      pi h (| cmd, argz |) /\
-      (forall (r:io_resm cmd) lt. (
-      (** postcondition **)
-//        ~(Inr? r /\ Inr?.v r == Contract_failure) /\
-        lt == [convert_call_to_event cmd argz r] /\
-        enforced_locally pi h lt)
-       ==>  p r lt)) =
-  IOwp?.reflect(fun _ _ -> io_call cmd argz)
+  (arg : io_sig.args cmd) :
+  IOPi (io_sig.res cmd arg) pi
+    (requires (fun h -> io_pre cmd arg h /\ pi h (| cmd, arg |)))
+    (ensures (fun h r lt ->
+        lt == [convert_call_to_event cmd arg r])) =
+  IOwp?.reflect (io_call cmd arg)
