io/Free.IO.Call.fst
@@ -1,14 +1,14 @@
 module Free.IO.Call
 
 open Free
-open Free.IO
+open Free.IO.Sig
 
 (** This file is replaced during linking with a file that contains the real
 implementation of the commands. **)
-let io_call (cmd:io_cmds) (arg:io_args cmd) : io (io_resm cmd) =
+let io_call (cmd:io_cmds) (arg:io_sig.args cmd) : io (io_sig.res cmd arg) =
   Call cmd arg Return
 
 (** Since we can lift from io to iio, `iio_call` should be used only for 
 `GetTrace`. **)
-let iio_call (cmd:inst_cmds) (arg:args cmd) : iio (res cmd) =
+let iio_call (cmd:cmds) (arg:iio_sig.args cmd) : iio (iio_sig.res cmd arg) =
   Call cmd arg Return
